progress on TypeCheck.v obligations

theories/Extraction/TypeCheck.v
@@ -61,8 +61,8 @@ Section type_check.
   | ti_zero : type_infer_order {{{ zero }}}
   | ti_succ : forall {M}, type_check_order M -> type_infer_order {{{ succ M }}}
   | ti_natrec : forall {A MZ MS M}, type_check_order M -> type_infer_order A -> type_check_order MZ -> type_check_order MS -> type_infer_order {{{ rec M return A | zero -> MZ | succ -> MS end }}}
-  | ti_pi : forall {s1 s2 s3} {r : Ru_pi P s1 s2 s3} {A B}, type_infer_order A -> type_infer_order B -> type_infer_order {{{ Π r A B }}}
-  | ti_fn : forall {s1 s2 s3} {r : Ru_pi P s1 s2 s3} {A B M}, type_infer_order A -> type_infer_order M -> type_infer_order {{{ λ r A B M }}}
+  | ti_pi : forall {s1 s2 s3} {r : Ru_pi P s1 s2 s3} {A B}, type_check_order A -> type_check_order B -> type_infer_order {{{ Π r A B }}}
+  | ti_fn : forall {s1 s2 s3} {r : Ru_pi P s1 s2 s3} {A B M}, type_check_order A -> type_check_order B -> type_check_order M -> type_infer_order {{{ λ r A B M }}}
   | ti_app : forall {M N}, type_infer_order M -> type_check_order N -> type_infer_order {{{ M N }}}
   | ti_vlookup : forall {x}, type_infer_order {{{ #x }}}
   .
@@ -82,31 +82,31 @@ Section type_check.
   #[local]
   Ltac clear_defs :=
     do 2 lazymatch goal with
-      | H: (forall (Γ : ctx ?P) (A : typ ?P),
+      | H: (forall (Γ : ?ctx) (A : ?expA),
                {{ Γ ⊢ A }} ->
-               forall M : typ ?P,
+               forall M : ?expM,
                  type_check_order M ->
                  ({ {{ Γ ⊢a M ⟸ A }} } + { ~ {{ Γ ⊢a M ⟸ A }} }))
         |- _ =>
           clear H
       | H: (let H := fixproto in
-            forall (P : PtsSig), (?dec_P : DecidableSig P) -> 
-            forall (Γ : ctx P) (A : typ P),
-              {{ Γ ⊢ A  }} -> forall M : typ P, type_check_order M -> { {{ Γ ⊢a M ⟸ A }} } + { ~ {{ Γ ⊢a M ⟸ A }} })
+            forall (P : PtsSig), (?dec_P : DecidableSig P) -> PredicativeSig P -> FunctionalSig P ->
+            forall (Γ : ?ctx) (A : ?expA),
+              {{ Γ ⊢ A }} -> forall M : ?expM, type_check_order M -> { {{ Γ ⊢a M ⟸ A }} } + { ~ {{ Γ ⊢a M ⟸ A }} })
         |- _ =>
           clear H
       | H: (let H := fixproto in
-            forall (P : PtsSig), (?dec_P : DecidableSig P) -> 
-            forall Γ : ctx P,
+            forall (P : PtsSig), DecidableSig P -> PredicativeSig P -> FunctionalSig P -> 
+            forall Γ : ?ctx,
               {{ ⊢ Γ }} ->
-              forall M : typ P,
+              forall M : ?expM,
                 type_infer_order M ->
                 ({ B : nf P | {{ Γ ⊢a M ⟹ B }} /\ {{ Γ ⊢aty ^(nf_to_exp B) }} } + { forall C : nf P, ~ {{ Γ ⊢a M ⟹ C }} }))
         |- _ =>
           clear H
-      | H: (forall Γ : ctx ?P,
+      | H: (forall Γ : ?ctx,
                {{ ⊢ Γ }} ->
-               forall M : typ ?P,
+               forall M : ?expM,
                  type_infer_order M ->
                  ({ B : nf ?P | {{ Γ ⊢a M ⟹ B }} /\{{ Γ ⊢aty ^(nf_to_exp B) }} } + { forall C : nf ?P, ~ {{ Γ ⊢a M ⟹ C }} }))
         |- _ =>
@@ -116,8 +116,8 @@ Section type_check.
   #[local]
   Ltac clear_redundant_pat :=
     repeat match goal with
-      | H: { A | {{ ^?Γ ⊢a ^?M ⟹ A }} /\ {{ ^?Γ ⊢aty A }} }
-          , H1: {{ ^?Γ ⊢a ^?M ⟹ ^?B }} /\ {{ ^?Γ ⊢aty ^?B }} |- _ => clear H
+      | H: { A | {{ ^?Γ ⊢a ^?M ⟹ A }} /\ {{ ^?Γ ⊢aty ^_ }} }
+          , H1: {{ ^?Γ ⊢a ^?M ⟹ ^?B }} /\ {{ ^?Γ ⊢aty ^_ }} |- _ => clear H
       | H: { s | ?A = n{{{ Sort@s }}} }
           , H1: ?A = n{{{ Sort@?s }}} |- _ => clear H
       | H: { B & { C | ?A = n{{{ Π ?r B C }}} } }
@@ -134,52 +134,51 @@ Section type_check.
   Ltac impl_obl_tac := clean_obl; eauto 3.
 
   #[tactic="impl_obl_tac",derive(equations=no,eliminator=no)]
-  Equations type_check {P : PtsSig} (dec_P : DecidableSig P) (Γ : ctx P) A (HA : {{ Γ ⊢ A }}) M (H : type_check_order M) : { {{ Γ ⊢a M ⟸ A }} } + { ~ {{ Γ ⊢a M ⟸ A }} } by struct H :=
-  | dec_P, Γ, A, HA, M, H =>
-      let*o->b (exist _ B _) := type_infer dec_P Γ _ M _ while _ in
+  Equations type_check {P : PtsSig} (dec_P : DecidableSig P) (pred_P : PredicativeSig P) (func_P : FunctionalSig P) (Γ : ctx P) A (HA : {{ Γ ⊢ A }}) M (H : type_check_order M) : { {{ Γ ⊢a M ⟸ A }} } + { ~ {{ Γ ⊢a M ⟸ A }} } by struct H :=
+  | dec_P, pred_P, func_P, Γ, A, HA, M, H =>
+      let*o->b (exist _ B _) := type_infer dec_P pred_P func_P Γ _ M _ while _ in
       let*b _ := subtyping_impl dec_P Γ (B : nf P) A _ while _ in
       pureb _
-  with type_infer {P : PtsSig} (dec_P : DecidableSig P) (Γ : ctx P) (HΓ : {{ ⊢ Γ }}) M (H : type_infer_order M) : { A : nf P | {{ Γ ⊢a M ⟹ A }} /\ {{ Γ ⊢aty A }} } + { forall A, ~ {{ Γ ⊢a M ⟹ A }} } by struct H :=
-  | dec_P, Γ, HΓ, M, H with M => {
+  with type_infer {P : PtsSig} (dec_P : DecidableSig P) (pred_P : PredicativeSig P) (func_P : FunctionalSig P) (Γ : ctx P) (HΓ : {{ ⊢ Γ }}) M (H : type_infer_order M) : { A : nf P | {{ Γ ⊢a M ⟹ A }} /\ {{ Γ ⊢aty A }} } + { forall A, ~ {{ Γ ⊢a M ⟹ A }} } by struct H :=
+  | dec_P, pred_P, func_P, Γ, HΓ, M, H with M => {
     | {{{ Sort@s }}} =>
-        (* pureo (exist _ n{{{ Sort@(S s) }}} _) *)
-        _ 
+        let*o (existT _ s' _) := dec_ax_typ dec_P s while _ in
+        pureo (exist _ n{{{ Sort@s' }}} _)
     | {{{ ℕ }}} =>
-    (* pureo (exist _ n{{{ Sort@0 }}} _) *)
-        _
+        let*o (existT _ s _) := dec_ru_nat dec_P while _ in
+        pureo (exist _ n{{{ Sort@s }}} _)
     | {{{ zero }}} =>
+        let*o (existT _ s _) := dec_ru_nat dec_P while _ in
         pureo (exist _ n{{{ ℕ }}} _)
     | {{{ succ M' }}} =>
-        let*b->o _ := type_check dec_P Γ {{{ ℕ }}} _ M' _ while _ in
+        let*o (existT _ s _) := dec_ru_nat dec_P while _ in
+        let*b->o _ := type_check dec_P pred_P func_P Γ {{{ ℕ }}} _ M' _ while _ in
         pureo (exist _ n{{{ ℕ }}} _)
     | {{{ rec M' return A' | zero -> MZ | succ -> MS end }}} =>
-        let*o (exist _ US _) := type_infer dec_P Γ _ {{{ ℕ }}} _ while _ in
-        let*o (exist _ s _) := get_level_of_sort_nf dec_P US while _ in
-        let*b->o _ := type_check dec_P Γ {{{ ℕ }}} _ M' _ while _ in
-        let*o (exist _ UA' _) := type_infer dec_P {{{ Γ, ℕ@s }}} _ A' _ while _ in
+        let*o (existT _ s _) := dec_ru_nat dec_P while _ in
+        let*o (exist _ UA' _) := type_infer dec_P pred_P func_P {{{ Γ, ℕ@s }}} _ A' _ while _ in
         let*o (exist _ s' _) :=  get_level_of_sort_nf dec_P UA' while _ in
-        let*b->o _ := type_check dec_P Γ {{{ A'[Id,,zero] }}} _ MZ _ while _ in
-        let*b->o _ := type_check dec_P {{{ Γ, ℕ@s, A'@s' }}} {{{ A'[Wk∘Wk,,succ #1] }}} _ MS _ while _ in
+        let*b->o _ := type_check dec_P pred_P func_P Γ {{{ A'[Id,,zero] }}} _ MZ _ while _ in
+        let*b->o _ := type_check dec_P pred_P func_P {{{ Γ, ℕ@s, A'@s' }}} {{{ A'[Wk∘Wk,,succ #1] }}} _ MS _ while _ in
+        let*b->o _ := type_check dec_P pred_P func_P Γ {{{ ℕ }}} _ M' _ while _ in
         let (A'', _) := nbe_ty_impl Γ {{{ A'[Id,,M'] }}} _ in
         pureo (exist _ A'' _)
     | {{{ Π r B C }}} =>
-        let*o (exist _ UB _) := type_infer dec_P Γ _ B _ while _ in
-        let*o (exist _ s _) :=  get_level_of_sort_nf dec_P UB while _ in
-        let*o (exist _ UC _) := type_infer dec_P {{{ Γ, B@s }}} _ C _ while _ in
-        let*o (exist _ j _) :=  get_level_of_sort_nf dec_P UC while _ in
-        (* pureo (exist _ n{{{ Sort@(max i j) }}} _) *)
-        _
+        let*b->o _ := type_check dec_P pred_P func_P Γ {{{ Sort@s1 }}} _ B _ while _ in
+        let*b->o _ := type_check dec_P pred_P func_P {{{ Γ, B@s1 }}} {{{ Sort@s2 }}} _ C _ while _ in
+        pureo (exist _ n{{{ Sort@s3 }}} _)
     | {{{ λ r A' B' M' }}} =>
-        let*o (exist _ UA' _) := type_infer dec_P Γ _ A' _ while _ in
-        let*o (exist _ s _) :=  get_level_of_sort_nf dec_P UA' while _ in
-        let*o (exist _ B' _) := type_infer dec_P  {{{ Γ, A'@s }}} _ M' _ while _ in
-        let (A'', _) := nbe_ty_impl Γ A' _ in
-        pureo (exist _ n{{{ Π r A'' B' }}} _)
+        let*b->o _ := type_check dec_P pred_P func_P Γ {{{ Sort@s4 }}} _ A' _ while _ in
+        let*b->o _ := type_check dec_P pred_P func_P {{{ Γ, A'@s4 }}} {{{ Sort@s5 }}} _ B' _ while _ in
+        let*b->o _ := type_check dec_P pred_P func_P {{{ Γ, A'@s4 }}} B' _ M' _ while _ in
+        let (A'', _) := nbe_impl Γ A' {{{ Sort@s4 }}} _ in
+        let (B'', _) := nbe_impl {{{ Γ, A'@s4 }}} B' {{{ Sort@s5 }}} _ in
+        pureo (exist _ n{{{ Π r A'' B'' }}} _)
     | {{{ M' N' }}} =>
-        let*o (exist _ C _) := type_infer dec_P Γ _ M' _ while _ in
+        let*o (exist _ C _) := type_infer dec_P pred_P func_P Γ _ M' _ while _ in
         let*o (existT _ s1 (existT _ s2 (existT _ s3 (existT _ r (existT _ A (exist _ B _)))))) :=
           get_subterms_of_pi_nf dec_P C while _ in
-        let*b->o _ := type_check dec_P Γ (A : nf P) _ N' _ while _ in
+        let*b->o _ := type_check dec_P pred_P func_P Γ (A : nf P) _ N' _ while _ in
         let (B', _) := nbe_ty_impl Γ {{{ ^(B : nf P)[Id,,N'] }}} _ in
         pureo (exist _ B' _)
     | {{{ #x }}} =>
@@ -208,7 +207,7 @@ Section type_check.
   #[local]
   Ltac impl_wf_context_obl_tac :=
     lazymatch goal with
-      | |- {{ ⊢ ^?Γ, ^?A }} =>
+      | |- {{ ⊢ ^?Γ, ^?A@^?s }} =>
           gen_presups;
           assert {{ ⊢ Γ }} by mauto 2;
           unshelve (eassert {{ Γ ⊢ A : ^n{{{ Sort@_ }}} }}; solve [mauto 2 using alg_type_infer_sound]); solve [constructor]
@@ -230,12 +229,13 @@ Section type_check.
     repeat match goal with
       | H: {{ ^?Γ ⊢a ^?M ⟹ ^?A }} |- _ => assert {{ Γ ⊢ M : A }} by eauto 2 using alg_type_infer_sound; fail_if_dup
       | H: {{ ^?Γ ⊢a ^?M ⟸ ^?A }} |- _ => assert {{ Γ ⊢ M : A }} by eauto 2 using alg_type_check_sound; fail_if_dup
+      | H: {{ ^?Γ ⊢aty ^?A }} |- _ => assert {{ Γ ⊢ A }} by eauto 2 using alg_aty_sound; fail_if_dup
       end.
 
   #[local]
   Ltac simplify_nbe_order :=
     lazymatch goal with
-    | |- nbe_ty_order ?Γ ?A => enough (exists i, {{ Γ ⊢ A : ^(nf_to_exp (nf_typ i)) }}) as [? [? []]%soundness_ty] by eauto 3 using nbe_ty_order_sound
+    | |- nbe_ty_order ?Γ ?A => enough ({{ Γ ⊢ A }}) as [? []]%soundness_ty by eauto 3 using nbe_ty_order_sound
     | |- nbe_order ?Γ ?M ?A => enough ({{ Γ ⊢ M : A }}) as [? []]%soundness by eauto 3 using nbe_order_sound
     end.
 
@@ -265,19 +265,18 @@ Section type_check.
         lazymatch goal with
         | |- nbe_ty_order ?Γ ?A =>
             simplify_nbe_order;
-            unshelve (eexists; solve [eauto 2]);
-            solve [constructor]
+            solve [eassumption]
         | |- nbe_order ?Γ ?M ?A =>
             simplify_nbe_order;
-            solve [eauto 2]
+            solve [eassumption]
         end
     end.
 
   #[local]
   Ltac impl_exist_lvl_wf_exp_obl_tac :=
     match goal with
-    | |- exists i, {{ ^?Γ ⊢ ^?A : Sort@i }} => enough (exists i, {{ Γ ⊢ A : ^(nf_to_exp (nf_typ i)) }}) by eauto 2
-    | |- exists i, {{ ^?Γ ⊢ ^?A : ^(nf_to_exp (nf_typ i)) }} => idtac
+    | |- exists s, {{ ^?Γ ⊢ ^?A : Sort@s }} => enough (exists s, {{ Γ ⊢ A : ^(nf_to_exp (nf_st s)) }}) by eauto 2
+    | |- exists s, {{ ^?Γ ⊢ ^?A : ^(nf_to_exp (nf_st s)) }} => idtac
     end;
     autoinjections;
     progressive_inversion;
@@ -307,228 +306,222 @@ Section type_check.
   Next Obligation.
     mautosolve 3.
   Qed.
+  
+  Next Obligation.
+    mautosolve 3.
+  Qed.
 
-  Next Obligation. (* exists j, {{ Γ ⊢ A'[Id,,zero] : Sort@j }} *)
-    eexists.
-    assert {{ ⊢ Γ, ℕ }} by mauto 3.
-    resolve_alg_sound.
+  Next Obligation.
+    dependent destruction H.
+    assert {{ Γ ⊢ B : Sort@s1 }} by mauto 3 using alg_type_check_sound.
     mauto 3.
   Qed.
 
-  Next Obligation. (* exists j, {{ Γ, ℕ, A' ⊢ A'[Wk∘Wk,,succ #1] : Sort@i }} *)
-    eexists.
-    assert {{ ⊢ Γ, ℕ }} by mauto 3.
-    resolve_alg_sound.
+  Next Obligation.
+    intros Hf.
+    inversion Hf; subst.
+    intuition.
+  Qed.
+
+  Next Obligation.
+    inversion H; mauto 2.
+  Qed.
+  
+  Next Obligation.
+    dependent destruction H.
+    assert {{ Γ ⊢ A' : Sort@s4 }} by mauto 3 using alg_type_check_sound.
     mauto 3.
   Qed.
 
-  Next Obligation. (* nbe_ty_order Γ {{{ A'[Id,,M'] }}} *)
-    simplify_nbe_order.
-    eexists.
-    assert {{ Γ ⊢ ℕ : Sort@0 }} by mauto 2.
-    assert {{ ⊢ Γ, ℕ }} by mauto 2.
-    resolve_alg_sound.
-    mauto 3.
+  Next Obligation.
+    intros Hf.
+    inversion Hf; subst.
+    intuition.
   Qed.
 
-  Next Obligation. (* {{ Γ ⊢a rec M' return A' | zero -> MZ | succ -> MS end ⟹ A'' }} /\ (exists j, {{ Γ ⊢a A'' ⟹ Sort@j }}) *)
-    split; [mautosolve 3 |].
-    assert {{ Γ ⊢ ℕ : Sort@0 }} by mauto 2.
-    assert {{ ⊢ Γ, ℕ }} by mauto 2.
-    resolve_alg_sound.
-    assert {{ Γ ⊢ A'[Id,,M'] : Sort@i }} by mauto 3.
-    assert {{ Γ ⊢ A'[Id,,M'] ≈ A'' : Sort@i }} by eauto 2 using soundness_ty'.
-    assert (user_exp A'') by trivial using user_exp_nf.
-    assert (exists j, {{ Γ ⊢a A'' ⟹ Sort@j }} /\ j <= i) as [? []] by (gen_presups; mauto 3).
-    eexists; eauto 2.
-  Qed.
-
-  Next Obligation. (* {{ Γ ⊢a λ A' M' ⟹ Π A'' B' }} /\ (exists j, {{ Γ ⊢a Π A'' B' ⟹ Sort@j }}) *)
-    split; [mautosolve 3 |].
-    resolve_alg_sound.
-    assert {{ ⊢ Γ, A' }} by mauto 2.
-    assert {{ Γ ⊢ A' ≈ A'' : Sort@i }} by eauto 2 using soundness_ty'.
-    assert {{ Γ ⊢ A'' : Sort@i }} by (gen_presups; mauto 2).
-    assert {{ ⊢ Γ, ^(A'' : exp) }} by mauto 2.
-    resolve_alg_sound.
-    assert {{ ⊢ Γ, A' ≈ Γ, ^(A'' : exp) }} by mauto 3.
-    eassert {{ Γ, ^(A'' : exp) ⊢ B' : Sort@_ }} by mauto 2.
-    assert (user_exp A'') by trivial using user_exp_nf.
-    assert (exists j, {{ Γ ⊢a A'' ⟹ Sort@j }} /\ j <= i) as [? []] by (gen_presups; mauto 2).
-    assert (user_exp B') by trivial using user_exp_nf.
-    eassert (exists k, {{ Γ, ^(A'' : exp) ⊢a B' ⟹ Sort@k }} /\ k <= H1) as [? []] by (gen_presups; mauto 2).
-    eexists; mauto 2.
-  Qed.
-
-  Next Obligation. (* nbe_ty_order Γ {{{ B[Id,,N'] }}} *)
-    simplify_nbe_order.
-    progressive_inversion.
-    resolve_alg_sound.
-    assert {{ ⊢ Γ, ^(A : exp) }} by mauto 2.
-    resolve_alg_sound.
-    eexists; mauto 3.
-  Qed.
-
-  Next Obligation. (* {{ Γ ⊢a M' N' ⟹ B' }} /\ (exists i, {{ Γ ⊢a B' ⟹ Sort@i }}) *)
-    progressive_inversion.
-    split; [mautosolve 3 |].
-    resolve_alg_sound.
-    assert {{ ⊢ Γ, ^(A : exp) }} by mauto 2.
-    resolve_alg_sound.
-    assert {{ Γ ⊢s Id,,N' : Γ, ^(A : exp) }} by mauto 2.
-    assert {{ Γ ⊢ B[Id,,N'] : ^n{{{ Sort@j }}} }} by mauto 2.
-    assert {{ Γ ⊢ B[Id,,N'] ≈ B' : Sort@j }} by mauto 2 using soundness_ty'.
-    assert (user_exp B') by trivial using user_exp_nf.
-    assert (exists k, {{ Γ ⊢a B' ⟹ Sort@k }} /\ k <= j) as [? []] by (gen_presups; mauto 2).
-    eexists; eauto 2.
-  Qed.
-
-  Next Obligation. (* exists i : nat, {{ Γ ⊢ B'[Id,,M1'] : Sort@i }} *)
-    progressive_inversion.
-    resolve_alg_sound.
-    assert {{ ⊢ Γ, A' }} by mauto 2.
-    resolve_alg_sound.
-    eexists; mauto 2.
-    eapply wf_conv'; [eapply wf_exp_sub |]; mauto 3.
-  Qed.
-
-  Next Obligation. (* nbe_ty_order {{{ Γ, A' }}} B' *)
-    progressive_inversion.
-    resolve_alg_sound.
-    simplify_nbe_order.
-    assert {{ ⊢ Γ, A' }} by mauto 2.
-    resolve_alg_sound.
-    eauto.
-  Qed.
-
-  Next Obligation. (* {{ Γ ⊢a ⟨ M1' : A'; M2' : B' ⟩ ⟹ Σ A'' B'' }} /\ (exists i0 : nat, {{ Γ ⊢a Σ A'' B'' ⟹ Sort@i0 }}) *)
-    progressive_inversion.
-    split; [mautosolve 3 |].
-    resolve_alg_sound.
-    assert {{ ⊢ Γ, A' }} by mauto 2.
-    resolve_alg_sound.
-    assert {{ Γ ⊢ A' ≈ A'' : Sort@i }} by mauto 2 using soundness_ty'.
-    assert {{ Γ ⊢ A'' : Sort@i }} by (gen_presups; mauto 2).
-    assert {{ Γ , A' ⊢ B' ≈ B'' : Sort@j }} by mauto 2 using soundness_ty'.
-    assert {{ Γ , A' ⊢ B'' : Sort@j }} by (gen_presups; mauto 2).
-    assert {{ Γ , ^(A'':typ) ⊢ B'' : Sort@j }} by (eapply @ctxeq_exp with (Γ:={{{Γ, A'}}}); mauto 3).
-    assert {{ Γ ⊢ Σ A'' B'' : Sort@(max i j) }} by mauto 2.
-    assert (user_exp n{{{ Σ A'' B'' }}}) by trivial using user_exp_nf.
-    eapply alg_type_infer_typ_complete in H57; mauto 3.
-    destruct_all. mauto 3.
-  Qed.
-
-  Next Obligation. (* {{ Γ ⊢a fst M' ⟹ A' }} /\ (exists i : nat, {{ Γ ⊢a A' ⟹ Sort@i }}) *)
-    progressive_inversion.
-    split; [mautosolve 3 |].
-    resolve_alg_sound.
-    assert (user_exp A') by trivial using user_exp_nf.
-    mauto.
-  Qed.
-
-  Next Obligation. (* nbe_ty_order Γ {{{ B[Id,,fst M'] }}} *)
-    progressive_inversion.
-    resolve_alg_sound.
-    simplify_nbe_order.
-    assert {{ Γ ⊢ fst M' : A' }} by mauto 2.
-    assert {{ ⊢ Γ, ^(A':typ) }} by mauto 2.
-    resolve_alg_sound.
-    eexists.
-    eapply wf_conv'; [eapply wf_exp_sub |]; mauto 3.
-  Qed.
-
-  Next Obligation.   (* {{ Γ ⊢a snd M' ⟹ B' }} /\ (exists i : nat, {{ Γ ⊢a B' ⟹ Sort@i0 }}) *)
-    progressive_inversion.
-    split; [mautosolve 3 |].
-    resolve_alg_sound.
-    mauto.
-    assert {{ Γ ⊢ fst M' : A' }} by mauto 2.
-    assert {{ ⊢ Γ, ^(A':typ) }} by mauto 2.
-    apply wf_sigma_inversion' in H12.
-    destruct_all.
-    assert {{ Γ ⊢ B[Id,,fst M'] ≈ B' : Sort@(max i j) }} by (eapply soundness_ty'; mauto 3).
-    gen_presups.
-    assert (user_exp B') by trivial using user_exp_nf.
-    eapply alg_type_infer_typ_complete in H18; mauto 3.
-    destruct_all. mauto 3.
-  Qed.
-
-  Next Obligation. (* {{ Γ ⊢a refl A' M' ⟹ Eq A'' M'' M'' }} /\ (exists i0 : nat, {{ Γ ⊢a Eq A'' M'' M'' ⟹ Sort@i0 }}) *)
-    split; [mautosolve 3 |].
-    resolve_alg_sound.
-    assert {{ Γ ⊢ A' ≈ A'' : Sort@i }} by eauto 2 using soundness_ty'.
-    assert {{ Γ ⊢ A' ≈ A'' : Sort@i }} by eauto 2 using soundness_ty'.
-    assert {{ Γ ⊢ M' ≈ M'' : A' }} by eauto 2 using soundness'.
-    assert {{ Γ ⊢ M' ≈ M'' : A'' }} by mauto 2.
-    assert {{ Γ ⊢ Eq A'' M'' M'' : Sort@i }} by (gen_presups; mauto 2).
-    assert (user_exp n{{{ Eq A'' M'' M'' }}}) by trivial using user_exp_nf.
-    assert (exists k, {{ Γ ⊢a Eq A'' M'' M'' ⟹ Sort@k }} /\ k <= i) as [? []] by (gen_presups; mauto 2).
-    eexists; eauto 2.
-  Qed.
-
-  Next Obligation. (* {{ ⊢ Γ, A', A'[Wk], Eq A'[Wk∘Wk] #1 #0 }} *)
-    resolve_alg_sound.
-    assert {{ Γ, A' ⊢s Wk : Γ }} by mauto 3.
-    assert {{ Γ, A' ⊢ A'[Wk] : Sort@i }} by mauto 2.
-    assert {{ ⊢ Γ, A', A'[Wk] }} by mauto 3.
-    assert {{ Γ, A', A'[Wk] ⊢ Eq A'[Wk∘Wk] #1 #0 : Sort@i }} by mauto 2.
+  Next Obligation.
+    assert {{ Γ ⊢ A' : Sort@s4 }} by mauto 3 using alg_type_check_sound.
+    assert {{ ⊢ Γ, A'@s4 }} by mauto 2.
+    assert {{ Γ, A'@s4 ⊢ B' : Sort@s5 }} by mauto 3 using alg_type_check_sound.
     mauto 2.
   Qed.
 
-  Next Obligation. (* exists i0 : nat, {{ Γ, A' ⊢ B'[Id,,#0,,refl A'[Wk] #0] : Sort@i0 }} *)
-    functional_alg_type_infer_rewrite_clear.
-    resolve_alg_sound.
-    assert {{ Γ, A' ⊢s Wk : Γ }} by mauto 3.
-    assert {{ Γ, A' ⊢ A'[Wk] : Sort@i }} by mauto 2.
-    assert {{ ⊢ Γ, A', A'[Wk] }} by mauto 3.
-    assert {{ Γ, A', A'[Wk] ⊢ Eq A'[Wk∘Wk] #1 #0 : Sort@i }} by mauto 2.
-    assert {{ Γ, A', A'[Wk], Eq A'[Wk∘Wk] #1 #0 ⊢ B' : ^n{{{ Sort@j }}} }} by mauto 3 using alg_type_infer_sound.
-    pose proof (@glu_rel_eq_eqrec_synprop_gen_A Γ {{{ Id }}} _ _ A' ltac:(mauto 2) ltac:(eassumption)).
-    destruct_all.
-    assert {{ Γ, A' ⊢ B'[Id,,#0,,refl A'[Wk] #0] : Sort@j }} by mauto 2.
-    eauto.
+  Next Obligation.
+    simplify_nbe_order.
+    mauto 3 using alg_type_check_sound.
   Qed.
 
-  Next Obligation. (* nbe_ty_order Γ {{{ B'[Id,,M1',,M2',,N'] }}} *)
+  Next Obligation.
+    simplify_nbe_order.
+    assert {{ Γ ⊢ A' : Sort@s4 }} by mauto 3 using alg_type_check_sound.
+    assert {{ ⊢ Γ, A'@s4 }} by mauto 2.
+    mauto 3 using alg_type_check_sound.
+  Qed.
+
+  Next Obligation.
+    split; [mautosolve 3|].
+    assert (user_exp P A'') by trivial using user_exp_nf.
+    assert (user_exp P B'') by trivial using user_exp_nf.    
+    enough {{ Γ ⊢ Π r A'' B'' : Sort@s6 }}; [eapply alg_aty_complete; mauto 2|].
+    assert {{ Γ ⊢ A' : Sort@s4 }} by mauto 3 using alg_type_check_sound.
+    assert {{ Γ, A'@s4 ⊢ B' : Sort@s5 }} by (eapply alg_type_check_sound; mauto 3).
+
+    assert {{ Γ ⊢ A' ≈ A'' : Sort@s4 }} by mauto 2 using soundness'.
+    assert {{ Γ, A'@s4 ⊢ B' ≈ B'' : Sort@s5 }} by mauto 2 using soundness'.
+    gen_presups.
+    assert {{ ⊢ Γ, A'@s4 ≈ Γ, ^(nf_to_exp A'')@s4 }} by mauto 3.
+    econstructor; mauto 2.
+  Qed.
+
+  Next Obligation.
+    dependent destruction H5.
+    dependent destruction H4.
+    dependent destruction H3.
+    dependent destruction H2.
+    dependent destruction H1.
+    dependent destruction e.
+    resolve_alg_sound.
+    simpl in H3.
+    gen_presups.
+    simpl in HAwf0.
+    eapply wf_typ_pi_inversion in HAwf0.
+    destruct_conjs.
+    mauto 2.
+  Qed.
+
+  Next Obligation.
+    dependent destruction H5.
+    dependent destruction H4.
+    dependent destruction H3.
+    dependent destruction H2.
+    dependent destruction e.
+    inversion a0; subst.
     simplify_nbe_order.
     resolve_alg_sound.
-    assert {{ Γ ⊢ Eq A' M1' M2' : Sort@i }} by mauto 2.
-    resolve_alg_sound.
-    assert {{ Γ, A' ⊢s Wk : Γ }} by mauto 3.
-    assert {{ Γ, A' ⊢ A'[Wk] : Sort@i }} by mauto 2.
-    assert {{ ⊢ Γ, A', A'[Wk] }} by mauto 3.
-    assert {{ Γ, A', A'[Wk] ⊢ Eq A'[Wk∘Wk] #1 #0 : Sort@i }} by mauto 2.
-    assert {{ Γ, A', A'[Wk], Eq A'[Wk∘Wk] #1 #0 ⊢ B' : ^n{{{ Sort@j }}} }} by mauto 3 using alg_type_infer_sound.
-    assert {{ Γ ⊢s Id,,M1',,M2',,N' : Γ, A', A'[Wk], Eq A'[Wk∘Wk] #1 #0 }} by mauto 2.
-    eexists; mauto 2.
+    eapply wf_typ_pi_inversion in H6.
+    destruct_conjs.
+    gen_presup H4.
+    assert {{ Γ ⊢ A0 ⊆ A }} by mauto 3 using alg_subtyping_sound.
+    assert {{ Γ ⊢ N' : A }} by mauto 2.
+    mauto 4.
   Qed.
 
-  Next Obligation. (* {{ Γ ⊢a eqrec N' as Eq A' M1' M2' return B' | refl -> BR' end ⟹ B'' }} /\ (exists i0 : nat, {{ Γ ⊢a B'' ⟹ Sort@i0 }}) *)
-    split; [mautosolve 3 |].
-    resolve_alg_sound.
-    assert {{ Γ ⊢ Eq A' M1' M2' : Sort@i }} by mauto 2.
-    resolve_alg_sound.
-    assert {{ Γ, A' ⊢s Wk : Γ }} by mauto 3.
-    assert {{ Γ, A' ⊢ A'[Wk] : Sort@i }} by mauto 2.
-    assert {{ ⊢ Γ, A', A'[Wk] }} by mauto 3.
-    assert {{ Γ, A', A'[Wk] ⊢ Eq A'[Wk∘Wk] #1 #0 : Sort@i }} by mauto 2.
-    assert {{ Γ, A', A'[Wk], Eq A'[Wk∘Wk] #1 #0 ⊢ B' : ^n{{{ Sort@j }}} }} by mauto 3 using alg_type_infer_sound.
-    assert {{ Γ ⊢s Id,,M1',,M2',,N' : Γ, A', A'[Wk], Eq A'[Wk∘Wk] #1 #0 }} by mauto 2.
-    assert {{ Γ ⊢ B'[Id,,M1',,M2',,N'] : Sort@j }} by mauto 2.
-    assert {{ Γ ⊢ B'[Id,,M1',,M2',,N'] ≈ B'' : Sort@j }} by eauto 2 using soundness_ty'.
-    assert (user_exp B'') by eauto 2 using user_exp_nf.
-    assert (exists k, {{ Γ ⊢a B'' ⟹ Sort@k }} /\ k <= j) as [? []] by (gen_presups; mauto 2).
-    eexists; eauto.
+  Next Obligation.
+    dependent destruction H5.
+    dependent destruction H4.
+    dependent destruction H3.
+    dependent destruction H2.
+    dependent destruction e.
+    split; [mautosolve 3|].
+    assert {{ Γ ⊢ Π r A B }} by (mauto 2 using alg_aty_sound).
+    eapply wf_typ_pi_inversion in H2 as [].
+    assert {{ Γ, ^(nf_to_exp A)@s1 ⊢ B }} by (gen_presups; mauto 2).
+    assert {{ Γ ⊢ N' : A }} by mauto 3 using alg_type_check_sound.
+    assert {{ Γ ⊢s Id,,N' : Γ, ^(nf_to_exp A)@s1 }} by mauto 2.
+    assert {{ Γ ⊢ B[Id,,N'] }} by mauto 2.
+    assert {{ Γ ⊢ B[Id,,N'] ≈ B' }} by mauto 2 using soundness_ty'.
+    assert (user_exp P B') by trivial using user_exp_nf.    
+    eapply alg_aty_complete; mauto 3.
+  Qed.  
+
+  Next Obligation.
+    simplify_nbe_order.
+    mauto 3.
   Qed.
 
-  Final Obligation. (* {{ Γ ⊢a #x ⟹ A' }} /\ (exists i, {{ Γ ⊢a A' ⟹ Sort@i }}) *)
-    split; [mautosolve 3 |].
-    assert (exists i, {{ Γ ⊢ A : Sort@i }}) as [i] by mauto 2.
+  Next Obligation.
+    split; [mautosolve 3|].
+    assert {{ Γ ⊢ A }} by mauto 3.
+    assert {{ Γ ⊢ A ≈ A' }} by mauto 2 using soundness_ty'.
+    assert (user_exp P A') by trivial using user_exp_nf.    
+    eapply alg_aty_complete; mauto 3.
+  Qed.
+
+  
+  Next Obligation.    
+    split; mautosolve 4.
+  Qed.
+
+  Next Obligation.
+    mautosolve 3.
+  Qed.
+
+  Next Obligation.
+    split; mautosolve 4.
+  Qed.
+
+  Next Obligation.
+    intros Hf.
+    inversion Hf; subst.
+    functional_alg_type_infer_rewrite_clear.
+    assert (s = s0) by (eapply Func_ru_nat; eassumption); subst.
+    intuition.
+  Qed.
+
+  Next Obligation.
+    intros Hf.
+    inversion Hf; subst.
+    assert (s = s0) by (eapply Func_ru_nat; eassumption); subst.
+    functional_alg_type_infer_rewrite_clear.
+    intuition.
+  Qed.
+  
+  Next Obligation.
+    assert {{ Γ ⊢ ℕ : Sort@s }} by mauto 2.
+    assert {{ ⊢ Γ, ℕ@s }} by mauto 2.
     resolve_alg_sound.
-    assert {{ Γ ⊢ A ≈ A' : Sort@i }} by eauto 2 using soundness_ty'.
-    assert (user_exp A') by trivial using user_exp_nf.
-    assert (exists j, {{ Γ ⊢a A' ⟹ Sort@j }} /\ j <= i) as [? []] by (gen_presups; mauto 2).
-    eexists; eauto 2.
+    simpl in *.
+    assert {{ Γ, ℕ@s ⊢ A' }} by mauto 2.
+    assert {{ Γ ⊢ zero : ℕ }} by mauto 2.
+    assert {{ Γ ⊢s Id,,zero : Γ, ℕ@s }} by mauto 2.
+    mauto 2.
+  Qed.
+
+  Next Obligation.
+    assert {{ Γ ⊢ ℕ : Sort@s }} by mauto 2.
+    assert {{ ⊢ Γ, ℕ@s }} by mauto 2.
+    resolve_alg_sound.
+    simpl in *.
+    assert {{ ⊢ Γ, ℕ@s, A'@s' }} by mauto 2.
+    assert {{ Γ ⊢s Id,,zero : Γ, ℕ@s }} by mauto 3.
+    assert {{ Γ ⊢ A'[Id,,zero] : Sort@s' }} by mauto 3.
+    assert {{ Γ, ℕ@s, A'@s' ⊢s Wk∘Wk : Γ }} by (econstructor; mauto 3).
+    assert {{ Γ, ℕ@s, A'@s' ⊢s Wk∘Wk,,succ #1 : Γ, ℕ@s }} by mauto 4.
+    assert {{ Γ, ℕ@s, A'@s' ⊢ A'[Wk∘Wk,,succ #1] : Sort@s' }} by mauto 4.
+    mauto 2.
+  Qed.
+
+  Next Obligation.
+  Admitted.
+
+  Next Obligation.
+    mautosolve 3.
+  Qed.
+  
+  Next Obligation.
+    simplify_nbe_order.
+    assert {{ Γ ⊢ ℕ : Sort@s }} by mauto 2.
+    assert {{ ⊢ Γ, ℕ@s }} by mauto 2.
+    resolve_alg_sound.
+    simpl in H4.
+    assert {{ Γ, ℕ@s ⊢ A' }} by mauto 2.
+    assert {{ Γ ⊢ M' : ℕ }} by mauto 3 using alg_type_check_sound.
+    assert {{ Γ ⊢s Id,,M' : Γ, ℕ@s }} by mauto 2.
+    mauto 3.
+  Qed.
+                
+  Final Obligation.
+    split; [mautosolve 3|].
+    assert {{ Γ ⊢ ℕ : Sort@s }} by mauto 2.
+    assert {{ ⊢ Γ, ℕ@s }} by mauto 2.
+    resolve_alg_sound.
+    simpl in H4.
+    assert {{ Γ ⊢ M' : ℕ }} by mauto 3 using alg_type_check_sound.
+    assert {{ Γ ⊢s Id,,M' : Γ, ℕ@s }} by mauto 2.
+    assert {{ Γ ⊢ A'[Id,,M'] }} by mauto 3.
+    assert {{ Γ ⊢ A'[Id,,M'] ≈ A'' }} by mauto 2 using soundness_ty'.
+    assert (user_exp P A'') by trivial using user_exp_nf.  
+    eapply alg_aty_complete; mauto 3.
   Qed.
 
   Extraction Inline type_check_functional type_infer_functional.
