theories/PtsSignature.v
@@ -134,12 +134,14 @@ Record DecidableSig (P : PtsSig) : Type :=
       dec_ru_pi: forall (s1 s2 s3 : P) (r : Ru_pi P s1 s2 s3) (r' : Ru_pi P s1 s2 s3),
         ( { r = r'} + {r <> r'} )%type;
       dec_st_sub : forall (s s' : P), ({st_subtyp s s'} + {~ st_subtyp s s'})%type;
-      dec_ru_nat : {s : P & {r : Ru_nat P s | True}} + (forall s, Ru_nat P s -> False);
+      dec_ru_nat : ({s & Ru_nat P s} + {forall s, Ru_nat P s -> False})%type;
+      dec_ax_typ : forall (s : P), ( {s' & Ax_typ P s s'} + {forall s', ~Ax_typ P s s'} )%type 
     }.
 Arguments dec_st {_}.
 Arguments dec_ru_pi {_}.
 Arguments dec_st_sub {_}.
 Arguments dec_ru_nat {_}.
+Arguments dec_ax_typ {_}.
 
 Section DecidableProperties.
   Context {P : PtsSig} (dec_P : DecidableSig P).
